code/hash/Hacl.Hash.MD5.fsti
@@ -5,6 +5,6 @@ open Spec.Hash.Definitions
 
 include Hacl.Hash.Core.MD5
 
-val update_multi: update_multi_st MD5
-val update_last: update_last_st MD5
-val hash: hash_st MD5
+val legacy_update_multi: update_multi_st MD5
+val legacy_update_last: update_last_st MD5
+val legacy_hash: hash_st MD5
